theories/ftlr/Cas.v
@@ -1,0 +1,28 @@
+From iris.proofmode Require Import tactics.
+From iris.program_logic Require Import weakestpre adequacy lifting.
+From stdpp Require Import base.
+From cap_machine Require Export logrel.
+From cap_machine.ftlr Require Import ftlr_base.
+From cap_machine.rules Require Import rules_CAS.
+Import uPred.
+
+
+Section fundamental.
+  Context {Σ:gFunctors} {memg:memG Σ} {regg:regG Σ}
+          `{MachineParameters}.
+
+  Notation D := ((leibnizO Word) -n> iPropO Σ).
+  Notation R := ((leibnizO Reg) -n> iPropO Σ).
+  Implicit Types w : (leibnizO Word).
+  Implicit Types interp : (D).
+
+
+  Lemma cas_case (r : leibnizO Reg) (p : Perm) (b e a : Addr) (w : Word)
+    (loc cond newvalue: RegName) (i: CoreN) P :
+    ftlr_instr r p b e a w (CAS loc cond newvalue) i P.
+  Proof.
+    intros Hp Hsome i' Hbae Hi.
+    iIntros "#IH #Hinv #Hinva #Hreg #[Hread Hwrite] Ha HP Hcls HPC Hmap".
+  Admitted.
+
+End fundamental.
