theories/rules/rules_CAS.v
@@ -1,0 +1,389 @@
+From iris.base_logic Require Export invariants gen_heap.
+From iris.program_logic Require Export weakestpre ectx_lifting.
+From iris.proofmode Require Import tactics.
+From iris.algebra Require Import frac.
+From cap_machine Require Export rules_base.
+
+Section cap_lang_rules.
+  Context `{memG Σ, regG Σ}.
+  Context `{MachineParameters}.
+  Implicit Types P Q : iProp Σ.
+  Implicit Types σ : ExecConf.
+  Implicit Types c : cap_lang.expr.
+  Implicit Types a b : Addr.
+  Implicit Types r : RegName.
+  Implicit Types v : cap_lang.val.
+  Implicit Types w : Word.
+  Implicit Types reg : gmap (CoreN * RegName) Word.
+  Implicit Types ms : gmap Addr Word.
+
+  Definition reg_allows_store (i: CoreN) (regs : Reg) (r : RegName) p b e a :=
+    regs !! (i, r) = Some (WCap p b e a) ∧
+    writeAllowed p = true ∧ withinBounds b e a = true.
+
+  Inductive Cas_failure_spec (i: CoreN) (regs: Reg)
+    (loc cond newvalue: RegName)
+    (mem : gmap Addr Word):=
+  | Cas_fail_const z:
+      regs !! (i, loc) = Some(WInt z) ->
+      Cas_failure_spec i regs loc cond newvalue mem
+  | Cas_fail_bounds p b e a:
+      regs !! (i, loc) = Some(WCap p b e a) ->
+      (writeAllowed p = false ∨ withinBounds b e a = false) →
+      Cas_failure_spec i regs loc cond newvalue mem
+  | Cas_fail_invalid_PC oldv:
+      incrementPC (<[ (i, cond) := oldv ]> regs) i = None ->
+      Cas_failure_spec i regs loc cond newvalue mem
+  .
+
+  Inductive Cas_spec (i: CoreN) (regs regs': Reg)
+    (loc cond newvalue: RegName)
+    (mem mem' : gmap Addr Word)
+    : cap_lang.val → Prop :=
+  | Cas_spec_failure:
+      regs = regs' ->
+      mem = mem' ->
+      Cas_failure_spec i regs loc cond newvalue mem  ->
+      Cas_spec i regs regs' loc cond newvalue mem mem' (i, FailedV)
+  | Cas_spec_success_eq p b e a (c oldv newv : Word) :
+      reg_allows_store i regs loc p b e a  →
+      mem !! a = Some oldv →
+      (* regs !! (i, cond) = Some oldv -> *)
+      (* regs !! (i, newvalue) = Some newv -> *)
+      oldv = c ->
+      mem' = (<[a := newv]> mem) →
+      incrementPC (<[ (i, cond) := oldv ]> regs) i = Some regs' ->
+      Cas_spec i regs regs' loc cond newvalue mem mem' (i, NextIV)
+  | Cas_spec_success_neq p b e a (c oldv newv : Word) :
+      reg_allows_store i regs loc p b e a  →
+      mem !! a = Some oldv →
+      (* regs !! (i, cond) = Some oldv -> *)
+      (* regs !! (i, newvalue) = Some newv -> *)
+      oldv ≠ c ->
+      incrementPC (<[ (i, cond) := oldv ]> regs) i = Some regs' ->
+      Cas_spec i regs regs' loc cond newvalue mem mem' (i, NextIV)
+.
+
+  Definition allow_store_map_or_true (i: CoreN) (r1 : RegName) (regs : Reg) (mem : gmap Addr Word):=
+    ∃ p b e a,
+      read_reg_inr regs i r1 p b e a ∧
+      if decide (reg_allows_store i regs r1 p b e a) then
+        ∃ w, mem !! a = Some w
+      else True.
+
+  Lemma allow_store_implies_storev:
+    ∀ (i: CoreN) (r1 : RegName)(r2 : RegName) (mem0 : gmap Addr Word) (r : Reg) (p : Perm) (b e a : Addr) storev,
+      allow_store_map_or_true i r1 r mem0
+      → r !! (i, r1) = Some (WCap p b e a)
+      → r !! (i, r2) = Some storev
+      → writeAllowed p = true
+      → withinBounds b e a = true
+      → ∃ (storev : Word),
+          mem0 !! a = Some storev.
+  Proof.
+    intros i r1 r2 mem0 r p b e a storev HaStore Hr2v Hwoa Hwa Hwb.
+    unfold allow_store_map_or_true in HaStore.
+    destruct HaStore as (?&?&?&?&[Hrr | Hrl]&Hwo).
+    - assert (Hrr' := Hrr).
+      rewrite Hrr in Hr2v; inversion Hr2v; subst.
+      case_decide as HAL.
+      * auto.
+      * unfold reg_allows_store in HAL.
+        destruct HAL. inversion Hwoa. auto.
+    - destruct Hrl as [z Hrl].  by congruence.
+  Qed.
+
+
+   Lemma wp_Cas Ep i
+     pc_p pc_b pc_e pc_a
+     (loc cond newvalue : RegName)
+     w mem regs :
+   decodeInstrW w = CAS loc cond newvalue →
+   isCorrectPC (WCap pc_p pc_b pc_e pc_a) →
+   regs !! (i, PC) = Some (WCap pc_p pc_b pc_e pc_a) →
+   regs_of_core (CAS loc cond newvalue) i ⊆ dom _ regs →
+   mem !! pc_a = Some w →
+   allow_store_map_or_true i loc regs mem → (* ???? *)
+
+   {{{ (▷ [∗ map] a↦w ∈ mem, a ↦ₐ w) ∗
+       ▷ [∗ map] k↦y ∈ regs, k ↦ᵣ y }}}
+     (i, Instr Executable) @ Ep
+   {{{ regs' mem' retv, RET retv;
+       ⌜ Cas_spec i regs regs' loc cond newvalue mem mem' retv⌝ ∗
+         ([∗ map] a↦w ∈ mem', a ↦ₐ w) ∗
+         [∗ map] k↦y ∈ regs', k ↦ᵣ y }}}.
+  Proof.
+     iIntros (Hinstr Hvpc HPC Dregs Hmem_pc HaStore φ) "(>Hmem & >Hmap) Hφ".
+     iApply wp_lift_atomic_head_step_no_fork; auto.
+     iIntros (σ1 l1 l2 n) "[Hr Hm] /=". destruct σ1; simpl.
+     iDestruct (gen_heap_valid_inclSepM with "Hr Hmap") as %Hregs.
+
+     (* Derive necessary register values in r *)
+     pose proof (lookup_weaken _ _ _ _ HPC Hregs).
+     specialize (indom_regs_incl _ _ _ Dregs Hregs) as Hri. unfold regs_of in Hri.
+     feed destruct (Hri i loc) as [locv [Hloc' Hloc]]. by set_solver+.
+     iDestruct (gen_mem_valid_inSepM mem m with "Hm Hmem") as %Hma; eauto.
+
+     iModIntro.
+     iSplitR. by iPureIntro; apply normal_always_head_reducible.
+     iNext. iIntros (e2 σ2 efs Hpstep).
+     apply prim_step_exec_inv in Hpstep as (-> & -> & (c & -> & Hstep)).
+     iSplitR; auto. eapply core_step_exec_inv in Hstep; eauto.
+
+     unfold exec in Hstep. simpl in Hstep.
+     rewrite Hloc in Hstep.
+
+
+     (* Now we start splitting on the different cases in the Cas spec, and prove them one at a time *)
+
+     destruct locv as  [| p b e a ] eqn:Hlocv.
+     { (* Failure: loc is not a capability *)
+       inversion Hstep as [Hs].
+       destruct (r !! (i, cond)), (r !! (i, newvalue)) ; cbn in Hs
+       ; simplify_eq.
+       all: cbn ; iFrame ; iApply "Hφ"; iFrame.
+       all: iPureIntro; econstructor; eauto; econstructor; eauto.
+     }
+
+     destruct (writeAllowed p && withinBounds b e a) eqn:HWA.
+     2 : { (* Failure: loc is either not within bounds or doesnt allow reading *)
+       apply andb_false_iff in HWA.
+       inversion Hstep as [Hs].
+       assert (HWA_neq: writeAllowed p && withinBounds b e a = false)
+         by (destruct HWA as [-> | ->]
+             ; [ apply andb_false_l | apply andb_false_r]
+             ; done).
+       rewrite HWA_neq in Hs ; clear HWA_neq.
+       destruct (r !! (i, cond)), (r !! (i, newvalue)), (m !! a)
+       ; cbn in Hs ; simplify_eq.
+       all: iFailWP "Hφ" Cas_fail_bounds.
+     }
+     apply andb_true_iff in HWA; destruct HWA as (Hwa & Hwb).
+     cbn in Hstep.
+
+     destruct (regs !! (i, cond)) as [c'|] eqn:HCV ; cbn in Hstep.
+     2: { destruct (Hri i cond) as [ ? [ Hrcond _ ] ].
+          rewrite /regs_of_core ; by set_solver +.
+          rewrite Hrcond in HCV ; inversion HCV.
+     }
+     apply (lookup_weaken regs r) in HCV as HCV' ; auto.
+     rewrite HCV' in Hstep ; cbn in Hstep.
+
+     destruct (regs !! (i, newvalue)) as [nv|] eqn:HNV ; cbn in Hstep.
+     2: { destruct (Hri i newvalue) as [ ? [ Hrnv _ ] ].
+          rewrite /regs_of_core ; by set_solver +.
+          rewrite Hrnv in HNV ; inversion HNV.
+     }
+     apply (lookup_weaken regs r) in HNV as HNV' ; auto.
+     rewrite HNV' in Hstep ; cbn in Hstep.
+
+     (* Prove that a is in the memory map now, otherwise we cannot continue *)
+     pose proof (allow_store_implies_storev i loc newvalue mem regs p b e a nv)
+       as (oldv & Hmema); auto.
+
+     (* Given this, prove that a is also present in the memory itself *)
+     iDestruct (gen_mem_valid_inSepM mem m a oldv with "Hm Hmem" ) as %Hma' ; auto.
+     rewrite Hma' in Hstep ; cbn in Hstep.
+     assert (Hwa_eq : writeAllowed p && withinBounds b e a = true)
+       by (apply andb_true_iff ; auto).
+     rewrite Hwa_eq in Hstep ; clear Hwa_eq.
+     destruct (decide (oldv = c')).
+     - (* oldv = c', the memory is modified *)
+       destruct (incrementPC (<[ (i, cond) := oldv ]> regs) i) as [ regs' |] eqn:Hregs'.
+      2: { (* Failure: the PC could not be incremented correctly *)
+        assert ((incrementPC (<[ (i, cond) := oldv ]> r) i) = None).
+        { eapply incrementPC_overflow_mono; first eapply Hregs'.
+          by rewrite lookup_insert_is_Some'; eauto.
+            by apply insert_mono; eauto. }
+        rewrite incrementPC_fail_updatePC /= in Hstep; auto.
+        simplify_eq.
+        iFailWP "Hφ" Cas_fail_invalid_PC.
+      }
+      simplify_eq.
+
+      iMod ((gen_mem_update_inSepM _ _ a) with "Hm Hmem") as "[Hm Hmem]" ; eauto.
+
+     (* Success *)
+      rewrite /update_mem /update_reg /= in Hstep.
+      Unshelve.
+      eapply (incrementPC_success_updatePC _ i (<[a:=nv]> m) ) in Hregs'
+        as (p1 & g1 & b1 & e1 & a1 & a_pc1 & HPC'' & HuPC & ->).
+      eapply (updatePC_success_incl i _ (<[a:=nv]> m)) in HuPC. 2: by eapply insert_mono.
+      rewrite HuPC in Hstep; clear HuPC; inversion Hstep; clear Hstep; subst c σ2. cbn.
+      iFrame.
+      iMod ((gen_heap_update_inSepM _ _ (i, cond)) with "Hr Hmap") as "[Hr Hmap]"; eauto.
+      iMod ((gen_heap_update_inSepM _ _ (i, PC)) with "Hr Hmap") as "[Hr Hmap]"; eauto.
+      iFrame. iModIntro. iApply "Hφ". iFrame.
+      iPureIntro. eapply Cas_spec_success_eq; eauto.
+        * split; auto. eassumption. all: auto.
+        * unfold incrementPC. by rewrite a_pc1 HPC''.
+
+     - (* oldv =! c', the memory is not modified *)
+     destruct (incrementPC (<[ (i, cond) := oldv ]> regs) i) as [ regs' |] eqn:Hregs'.
+      2: { (* Failure: the PC could not be incremented correctly *)
+        assert ((incrementPC (<[ (i, cond) := oldv ]> r) i) = None).
+        { eapply incrementPC_overflow_mono; first eapply Hregs'.
+          by rewrite lookup_insert_is_Some'; eauto.
+            by apply insert_mono; eauto. }
+        rewrite incrementPC_fail_updatePC /= in Hstep; auto.
+        simplify_eq.
+        iFailWP "Hφ" Cas_fail_invalid_PC.
+      }
+
+     (* Success *)
+      rewrite /update_mem /update_reg /= in Hstep.
+      Unshelve.
+      eapply (incrementPC_success_updatePC _ i m) in Hregs'
+        as (p1 & g1 & b1 & e1 & a1 & a_pc1 & HPC'' & HuPC & ->).
+      eapply (updatePC_success_incl i _ m) in HuPC.
+      2: by eapply insert_mono.
+      rewrite HuPC in Hstep; clear HuPC; inversion Hstep; clear Hstep; subst c σ2. cbn.
+      iFrame.
+      iMod ((gen_heap_update_inSepM _ _ (i, cond)) with "Hr Hmap") as "[Hr Hmap]"; eauto.
+      iMod ((gen_heap_update_inSepM _ _ (i, PC)) with "Hr Hmap") as "[Hr Hmap]"; eauto.
+      iFrame. iModIntro. iApply "Hφ". iFrame.
+      iPureIntro. eapply Cas_spec_success_neq; eauto.
+        * split; auto. eassumption. all: auto.
+        * unfold incrementPC. by rewrite a_pc1 HPC''.
+   Qed.
+
+    Lemma mem_eq_implies_allow_store_map:
+    ∀ (i: CoreN)(regs : Reg)(mem : gmap Addr Word)(r1 : RegName)(w : Word) p b e a,
+      mem = <[a:=w]> ∅
+      → regs !! (i, r1) = Some (WCap p b e a)
+      → allow_store_map_or_true i r1 regs mem.
+  Proof.
+    intros i regs mem r1 w p b e a Hmem Hrr2.
+    exists p,b,e,a; split.
+    - left. by simplify_map_eq.
+    - case_decide; last done.
+      exists w. simplify_map_eq. auto.
+  Qed.
+
+  Lemma mem_neq_implies_allow_store_map:
+    ∀ (i: CoreN)(regs : Reg)(mem : gmap Addr Word)(r1 : RegName)(pc_a : Addr)
+      (w w' : Word) p b e a,
+      a ≠ pc_a
+      → mem = <[pc_a:=w]> (<[a:=w']> ∅)
+      → regs !! (i, r1) = Some (WCap p b e a)
+      → allow_store_map_or_true i r1 regs mem.
+  Proof.
+    intros i regs mem r1 pc_a w w' p b e a H4 Hrr2.
+    exists p,b,e,a; split.
+    - left. by simplify_map_eq.
+    - case_decide; last done.
+      exists w'. simplify_map_eq. split; auto.
+  Qed.
+
+
+
+    Lemma mem_implies_allow_store_map:
+    ∀ (i: CoreN)(regs : Reg)(mem : gmap Addr Word)(r1 : RegName)(pc_a : Addr)
+      (w w' : Word) p b e a,
+      (if (a =? pc_a)%a
+       then mem = <[pc_a:=w]> ∅
+       else mem = <[pc_a:=w]> (<[a:=w']> ∅))
+      → regs !! (i, r1) = Some (WCap p b e a)
+      → allow_store_map_or_true i r1 regs mem.
+  Proof.
+    intros i regs mem r1 pc_a w w' p b e a H4 Hrr2.
+    destruct (a =? pc_a)%a eqn:Heq.
+      + apply Z.eqb_eq, finz_to_z_eq in Heq. subst a. eapply mem_eq_implies_allow_store_map; eauto.
+      + apply Z.eqb_neq in Heq.  eapply mem_neq_implies_allow_store_map; eauto. congruence.
+  Qed.
+
+
+
+  Lemma wp_cas_success_eq
+    E i r1 r2 r3
+    pc_p pc_b pc_e pc_a pc_a'
+    instr p b e a oldv cond newv
+    :
+   decodeInstrW instr = CAS r1 r2 r3 →
+   isCorrectPC (WCap pc_p pc_b pc_e pc_a) →
+   oldv = cond ->
+   (pc_a + 1)%a = Some pc_a' →
+   writeAllowed p = true → withinBounds b e a = true →
+
+    {{{ ▷ (i, PC) ↦ᵣ WCap pc_p pc_b pc_e pc_a
+        ∗ ▷ pc_a ↦ₐ instr
+        ∗ ▷ (i, r1) ↦ᵣ (WCap p b e a)
+        ∗ (if (eqb_addr a pc_a) then emp else ▷ a ↦ₐ oldv)
+        ∗ ▷ (i, r2) ↦ᵣ cond
+        ∗ ▷ (i, r3) ↦ᵣ newv }}}
+      (i, Instr Executable) @ E
+      {{{ RET (i, NextIV);
+          (i, PC) ↦ᵣ WCap pc_p pc_b pc_e pc_a'
+        ∗ pc_a ↦ₐ (if (a =? pc_a)%a then newv else instr)
+        ∗ (i, r1) ↦ᵣ (WCap p b e a)
+        ∗ (if (eqb_addr a pc_a) then emp else ▷ a ↦ₐ newv)
+        ∗ (i, r2) ↦ᵣ oldv
+        ∗ (i, r3) ↦ᵣ newv }}}.
+  (* TODO *)
+   Proof.
+     intros. iIntros "(>HPC & >Hpc_a & Hr1 & Hloc & Hr2 & Hr3) Hφ".
+     iDestruct (map_of_regs_4 with "HPC Hr1 Hr2 Hr3") as ">[Hmap Hregs]".
+     iDestruct "Hregs" as "[% [% [% [% [% %]]]]]".
+     iDestruct (memMap_resource_2gen_clater pc_a a _ _ (λ a w, a ↦ₐ w)%I  with
+                 "Hpc_a Hloc")
+       as (mem) "[Hmem %]".
+
+    iApply (wp_Cas with "[$Hmap $Hmem]"); eauto
+    ; simplify_map_eq by simplify_pair_eq; eauto.
+    { rewrite /regs_of_core ; set_solver. }
+    { destruct (a =? pc_a)%a; by simplify_map_eq by simplify_pair_eq. }
+    { eapply mem_implies_allow_store_map; eauto.
+      all : by simplify_map_eq by simplify_pair_eq. }
+    iModIntro.
+    iIntros (regs' mem' retv) "[#Hspec [Hmem Hregs]]".
+    iDestruct "Hspec" as %Hspec.
+    inversion Hspec ; subst.
+    - (* Failure *)
+      destruct H16; try incrementPC_inv; simplify_map_eq by simplify_pair_eq; eauto.
+       destruct o. all: congruence.
+    - (* Success with equality *)
+      iApply "Hφ".
+      destruct H4 as [Hrr2 _]. simplify_map_eq by simplify_pair_eq.
+     (*  destruct ( decide (a0 = pc_a)) *)
+     (*  ; simplify_eq *)
+     (*  ; subst. *)
+     (*  + (* a0 = pc_a *) *)
+     (*  rewrite Z.eqb_refl in H14 ; rewrite Z.eqb_refl. *)
+     (*  subst. *)
+     (*  rewrite memMap_resource_1. *)
+     (*   incrementPC_inv. *)
+     (*   simplify_map_eq by simplify_pair_eq. *)
+     (*   rewrite (insert_commute _ (i, PC) (i, r2)) ; simplify_pair_eq. *)
+     (*   rewrite insert_insert insert_insert. *)
+     (*   rewrite (insert_commute _ (i, r2) (i, PC)) ; simplify_pair_eq. *)
+     (*   rewrite (insert_commute _ (i, r2) (i, r1)) ; simplify_pair_eq. *)
+     (*   rewrite insert_insert. *)
+     (*   iDestruct (regs_of_map_4 with "[$Hregs]") as "(HPC & Hr1 & Hr2 & Hr3)" *)
+     (*   ; eauto. iFrame. *)
+
+     (*   destruct ( (a0 =? x2)%Z ) eqn:Heq_addr *)
+     (*   ; [ rewrite -> Z.eqb_eq in Heq_addr | rewrite -> Z.eqb_neq in Heq_addr ] *)
+     (*   ; subst *)
+     (*   ; simplify_eq. *)
+     (*   apply lookup_insert_Some in H15 ; destruct H15 as [ [? ?]|?]. *)
+     (*   simplify_eq. *)
+     (*   iFrame. *)
+     (*   rewrite lookup_insert in H15. *)
+
+
+     (* } iFrame. *)
+
+     (*  iFrame. *)
+
+     (*  (* Failure *) *)
+
+
+
+
+     (* iApply (wp_store_success_reg' with "[$HPC $Hpc_a $Hdst]"); eauto. *)
+     (* { rewrite Z.eqb_refl. eauto. } *)
+     (* iNext. iIntros "(? & ? & ? & ?)". rewrite Z.eqb_refl. *)
+     (* iApply "Hφ". iFrame. Unshelve. eauto. *)
+   Admitted.
+
+End cap_lang_rules.
